LtlFrp/FRP/Hoare.lean
@@ -1,6 +1,19 @@
-import LtlFrp.FRP.Refining
+import LtlFrp.FRP.Verified
 
-namespace FRP.Refining
+namespace FRP
+
+-- ANCHOR: hoare
+abbrev Hoare (P : StateProp α) (Q : StateProp β):=
+  (□ α // P) → (□ β // Q)
+
+infixr:35 " ⟹ " => Hoare
+-- ANCHOR_END: hoare
+
+-- ANCHOR: refined-value-syntax
+syntax "⦃" ident " : " term " // " term "⦄" : term
+macro_rules
+  | `(⦃$i:ident : $ty // $p⦄) => `((fun $i : $ty => $p : StateProp $ty))
+-- ANCHOR_END: refined-value-syntax
 
 -- ANCHOR: hoare-skip
 def hoare_skip {P : StateProp α} : ⦃ a : α // P a ⦄ ⟹ ⦃ a : α // P a ⦄ :=
@@ -14,26 +27,16 @@ def hoare_seq {P : StateProp α} {Q : StateProp β} {R : StateProp γ} :
     (⦃a : α // P a⦄ ⟹ ⦃c : γ // R c⦄) := Function.comp
 -- ANCHOR_END: hoare-seq
 
--- ANCHOR: hoare-if-val
-def hoare_if_val
+-- ANCHOR: hoare-if
+def hoare_if
   {P : StateProp α} {Q : StateProp β}
   (C : StateProp α) [inst : DecidablePred C]
   (thn : {a : α // P a ∧ C a}   → {b : β // Q b})
   (els : {a : α // P a ∧ ¬ C a} → {b : β // Q b})
-  (a : {a : α // P a})
-  : {b : β // Q b} :=
-  if h : C a.val
-  then thn ⟨a.val, And.intro a.property h⟩
-  else els ⟨a.val, And.intro a.property h⟩
--- ANCHOR_END: hoare-if-val
-
--- ANCHOR: hoare-if
-def hoare_if
-  (C : StateProp α) [inst : DecidablePred C]
-  (thn : {a : α // P a ∧ C a}   → {b : β // Q b})
-  (els : {a : α // P a ∧ ¬ C a} → {b : β // Q b})
-  (input : □ α // P)
-  : □ β // Q := hoare_if_val C thn els <$$> input
+  : (⦃a : α // P a⦄ ⟹ ⦃b : β // Q b⦄) := fun sig =>
+  (fun ⟨val, prop⟩ => if h : C val
+    then thn ⟨val, And.intro prop h⟩
+    else els ⟨val, And.intro prop h⟩) <$$> sig
 -- ANCHOR_END: hoare-if
 
 -- ANCHOR: iter-one
@@ -48,14 +51,15 @@ def Event.when
   (P : StateProp α)
   (raise : StateProp α) [DecidablePred raise]
   (sig : □ α // P)
-  (hTerm : ∃ t, raise (sig.val t))
+  (hLive : (◇ ⌜raise⌝) sig.val)      -- ◇: `raise` eventually holds
   : ◇ {a : α // P a ∧ raise a} :=
+    have hTerm : ∃ t, raise (sig.val t) := (eventually_atom_iff sig.val).mpr hLive
     let toOpt : {a : α // P a} → Option {a : α // P a ∧ raise a} :=
       fun ⟨a, hp⟩ => if h : raise a then some ⟨a, And.intro hp h⟩ else none
     let f : □ (Option {a : α // P a ∧ raise a}) := toOpt <$> sig
     have live : FRP.fires f := by
       unfold FRP.fires
-      simp [toOpt, f, Functor.map, FRP.Refining.Signal.split]
+      simp [toOpt, f, Functor.map, FRP.RSignal.split]
       exact hTerm
     { f, live }
 -- ANCHOR_END: event-when
@@ -65,8 +69,8 @@ def RSignal.while
   (P b : StateProp α)           -- P, our loop invariant; b, our loop check
   [inst : DecidablePred b]
   (s : □ α // P)                -- our source of input values to poll
-  (hTerm : ∃ t, ¬ b (s.val t))  -- Proof that we eventually exit the loop
-  : ◇ {a : α // P a ∧ ¬b a} := Event.when P (¬b ·) s hTerm
+  (hLive : (◇ ⌜(¬b ·)⌝) s.val)  -- ◇: we eventually exit the loop
+  : ◇ {a : α // P a ∧ ¬b a} := Event.when P (¬b ·) s hLive
 -- ANCHOR_END: rsignal-while
 
-end FRP.Refining
+end FRP
